meta-theory/pure_demandScript.sml
@@ -1759,11 +1759,11 @@ Datatype:
        | RecBind ((string # exp) list) ctxt
 End
 
-Definition apply_ctxt_def:
-  apply_ctxt Nil e = e ∧
-  apply_ctxt (IsFree s c) e = apply_ctxt c (Lam s e) ∧
-  apply_ctxt (Bind s e1 c) e2 = apply_ctxt c (Let s e1 e2) ∧
-  apply_ctxt (RecBind l c) e = apply_ctxt c (Letrec l e)
+Definition exp_eq_in_ctxt_def:
+  exp_eq_in_ctxt Nil = (λe1 e2. e1 ≈ e2) ∧
+  exp_eq_in_ctxt (IsFree s c) e1 e2 = (∀e3. closed e3 ⇒ exp_eq_in_ctxt c (Let s e3 e1) (Let s e3 e2)) ∧
+  exp_eq_in_ctxt (Bind s e3 c) e1 e2 = exp_eq_in_ctxt c (Let s e3 e1) (Let s e3 e2) ∧
+  exp_eq_in_ctxt (RecBind l c) e1 e2 = exp_eq_in_ctxt c (Letrec l e1) (Letrec l e2)
 End
 
 Definition ctxt_size_def:
@@ -1862,7 +1862,7 @@ Inductive find: (* i i o o *)
      ⇒ find (Let v e e2) c ds'' (Let v e' e2')) ∧
 [find_Lam:]
   (∀e e' c ds v.
-     find e c ds e' ⇒ find (Lam v e) c {} (Lam v e')) ∧
+     find e (IsFree v c) ds e' ⇒ find (Lam v e) c {} (Lam v e')) ∧
 [find_Lams:]
   (∀e e' c ds vl.
      find e (FOLDL (λc n. IsFree n c) c vl) ds e' ⇒ find (Lams vl e) c {} (Lams vl e')) ∧
@@ -1872,38 +1872,406 @@ Inductive find: (* i i o o *)
   (∀e e' ds c b b'. LIST_REL (λ(n1, e1) (n2, e2). n1 = n2 ∧ e1 ≈ e2) b b' ∧ find e (RecBind b c) ds e' ⇒ find (Letrec b e) c {} (Letrec b e'))
 End
 
-Theorem exp_eq_apply_ctxt_cong:
-  ∀c e e'. e ≈ e' ⇒ apply_ctxt c e ≈ apply_ctxt c e'
+Theorem exp_eq_in_ctxt_refl:
+  ∀c e. exp_eq_in_ctxt c e e
 Proof
   Induct
-  \\ gvs [apply_ctxt_def]
-  \\ rw []
-  \\ last_x_assum $ irule
-  \\ gvs [exp_eq_Lam_cong, exp_eq_App_cong, exp_eq_Letrec_cong, exp_eq_refl, exp_eq_l_refl]
+  \\ gvs [exp_eq_in_ctxt_def, exp_eq_refl]
 QED
 
-Theorem exp_eq_apply_ctxt_push:
-  ∀c e1 e2 e3 e4. (e1 ≈ e2 ⇒ e3 ≈ e4) ∧ apply_ctxt c e1 ≈ apply_ctxt c e2 ⇒ apply_ctxt c e3 ≈ apply_ctxt c e4
+Theorem exp_eq_in_ctxt_sym:
+  ∀c e1 e2. exp_eq_in_ctxt c e1 e2 ⇔ exp_eq_in_ctxt c e2 e1
 Proof
   Induct
-  \\ gvs [apply_ctxt_def]
+  \\ rw [] \\ eq_tac
+  \\ gvs [exp_eq_in_ctxt_def, exp_eq_sym]
+QED
+
+Theorem exp_eq_in_ctxt_trans:
+  ∀c e1 e2 e3. exp_eq_in_ctxt c e1 e2 ∧ exp_eq_in_ctxt c e2 e3 ⇒ exp_eq_in_ctxt c e1 e3
+Proof
+  Induct
   \\ rw []
-  \\ last_x_assum $ irule
-  \\ pop_assum $ irule_at Any
-  \\ strip_tac
-  >- (irule exp_eq_Lam_cong \\ first_x_assum irule
-      \\ gvs [exp_eq_open_bisimilarity_freevars, open_bisimilarity_eq, open_similarity_def, app_similarity_iff]
-      \\ rw [bind_def] \\ fs [] >>~[‘(Fail, Fail)’]
-      >- rw [unfold_rel_def, eval_wh_Fail]
-      >- rw [unfold_rel_def, eval_wh_Fail]
-      \\ ‘∀v. v ∈ FRANGE f ⇒ closed v’ by (rw [] \\ first_x_assum irule
-                                           \\ fs [FRANGE_FLOOKUP] \\ first_x_assum $ irule_at Any)
-      \\ dxrule_then assume_tac IMP_closed_subst
-      \\ first_assum dxrule
+  \\ gvs [exp_eq_in_ctxt_def]
+  >- (irule exp_eq_trans
+      \\ pop_assum $ irule_at Any \\ fs [])
+  \\ rw []
+  \\ last_x_assum irule
+  \\ first_x_assum $ irule_at Any
+  \\ gvs []
+QED
+
+Theorem exp_eq_IMP_exp_eq_in_ctxt:
+  ∀c e e'. e ≈ e' ⇒ exp_eq_in_ctxt c e e'
+Proof
+  Induct
+  \\ gvs [exp_eq_in_ctxt_def]
+  \\ rw []
+  \\ first_x_assum irule
+  \\ gvs [exp_eq_Letrec_cong, exp_eq_App_cong, exp_eq_Lam_cong, exp_eq_refl, exp_eq_l_refl]
+QED
+
+Theorem eval_Prim:
+  ∀ope eL eL'. LIST_REL (λe1 e2. eval e1 = eval e2) eL eL' ⇒ eval (Prim ope eL) = eval (Prim ope eL')
+Proof
+  Cases
+  \\ rw [eval_thm]
+  >~[‘MAP _ _ = MAP _ _’]
+  >- (irule LIST_EQ
+      \\ gvs [LIST_REL_EL_EQN, EL_MAP])
+  >~[‘AtomOp’]
+  >- (fs [eval_def]
+      \\ once_rewrite_tac [v_unfold]
+      \\ fs [eval_wh_Prim]
+      \\ qsuff_tac ‘get_atoms (MAP eval_wh eL') = get_atoms (MAP eval_wh eL)’
+      >- (CASE_TAC \\ fs [])
+      \\ fs [get_atoms_def]
+      \\ qsuff_tac ‘EXISTS error_Atom (MAP eval_wh eL) ⇔ EXISTS error_Atom (MAP eval_wh eL')’
+      >- (strip_tac
+          \\ IF_CASES_TAC
+          \\ simp []
+          \\ qsuff_tac ‘MEM wh_Diverge (MAP eval_wh eL) ⇔ MEM wh_Diverge (MAP eval_wh eL')’
+          >- (strip_tac
+              \\ IF_CASES_TAC
+              \\ simp []
+              \\ irule LIST_EQ
+              \\ rw []
+              \\ gvs [LIST_REL_EL_EQN, EL_MAP, EVERY_EL]
+              \\ rpt $ first_x_assum drule
+              \\ once_rewrite_tac [v_unfold]
+              \\ rpt FULL_CASE_TAC
+              \\ rw [dest_Atom_def, error_Atom_def])
+          \\ eq_tac
+          \\ strip_tac
+          \\ gvs [MEM_EL, LIST_REL_EL_EQN]
+          \\ first_assum $ irule_at Any
+          \\ first_assum drule
+          \\ once_rewrite_tac [v_unfold]
+          \\ rpt FULL_CASE_TAC
+          \\ gvs [EL_MAP])
+      \\ eq_tac
+      \\ strip_tac
+      \\ gvs [EXISTS_MEM, MEM_EL, EL_MAP, LIST_REL_EL_EQN]
+      \\ rename1 ‘MAP eval_wh eL2’
+      \\ qexists_tac ‘eval_wh (EL n eL2)’
+      \\ first_x_assum drule
+      \\ once_rewrite_tac [v_unfold]
+      \\ rpt FULL_CASE_TAC
+      \\ fs [error_Atom_def]
+      \\ rw []
+      \\ first_assum $ irule_at Any
+      \\ fs [EL_MAP])
+  \\ Cases_on ‘eL’ \\ Cases_on ‘eL'’ \\ fs []
+  \\ rename1 ‘LIST_REL _ t1 t2’
+  \\ Cases_on ‘t1’ \\ Cases_on ‘t2’ \\ gvs [eval_thm]
+  >~[‘Prim Seq (_::_::_)’]
+  >- (rename1 ‘LIST_REL _ t1 t2’
+      \\ Cases_on ‘t1’ \\ Cases_on ‘t2’
+      \\ gvs [eval_thm, eval_def]
+      \\ once_rewrite_tac [v_unfold]
+      \\ fs [eval_wh_Prim])
+  >~[‘Prim If (_::_::_)’]
+  >- (rename1 ‘LIST_REL _ t1 t2’
+      \\ Cases_on ‘t1’ \\ Cases_on ‘t2’ \\ gvs []
+      >~[‘_::_::_::_’]
+      >- (rename1 ‘LIST_REL _ t1 t2’
+          \\ Cases_on ‘t1’ \\ Cases_on ‘t2’
+          \\ gvs [eval_thm, eval_def]
+          \\ once_rewrite_tac [v_unfold]
+          \\ rw [eval_wh_Prim])
+      \\ rw [eval_def]
+      \\ once_rewrite_tac [v_unfold]
+      \\ rw [eval_wh_Prim])
+  \\ rw [eval_def]
+  \\ once_rewrite_tac [v_unfold]
+  \\ rw [eval_wh_Prim]
+QED
+
+Theorem FLOOKUP_LUPDATE:
+  ∀l f n v. FLOOKUP (f |++ l) n = SOME v ⇒ MEM (n, v) l ∨ FLOOKUP f n = SOME v
+Proof
+  Induct
+  \\ fs [FUPDATE_LIST_THM]
+  \\ PairCases \\ rw []
+  \\ first_x_assum $ dxrule_then assume_tac
+  \\ gvs [FLOOKUP_UPDATE]
+  \\ FULL_CASE_TAC \\ fs []
+QED
+
+Theorem Letrec_Prim:
+  ∀l ope eL b. (Letrec l (Prim ope eL) ≅? Prim ope (MAP (Letrec l) eL)) b
+Proof
+  rw []
+  \\ irule eval_IMP_exp_eq
+  \\ rw [subst_def, eval_thm, subst_funs_def, bind_def]
+  >- (irule eval_Prim
+      \\ rw [LIST_REL_EL_EQN, EL_MAP, subst_def, eval_thm, subst_funs_def]
+      \\ gvs [bind_def]
+      \\ IF_CASES_TAC \\ fs []
       \\ first_x_assum dxrule
-      \\ rw [unfold_rel_def]
+      \\ strip_tac
+      \\ fs [])
+  \\ fs [MAP_MAP_o]
+  \\ dxrule_then assume_tac FLOOKUP_LUPDATE
+  \\ gvs [FLOOKUP_EMPTY, MEM_EL, EL_MAP]
+  \\ qsuff_tac ‘F’ \\ fs []
+  \\ first_x_assum irule
+  \\ rename1 ‘EL k l’
+  \\ qabbrev_tac ‘p = EL k l’
+  \\ PairCases_on ‘p’
+  \\ gvs [EVERY_EL, EL_MAP]
+  \\ rw []
+  \\ rename1 ‘EL k2 l’
+  \\ qabbrev_tac ‘p' = EL k2 l’
+  \\ PairCases_on ‘p'’
+  \\ gvs []
+  \\ ‘∀v. v ∈ FRANGE (FDIFF f (set (MAP FST l))) ⇒ closed v’
+    by (rw []
+        \\ first_x_assum irule
+        \\ gvs [FRANGE_FLOOKUP, FLOOKUP_FDIFF]
+        \\ pop_assum $ irule_at Any)
+  \\ gvs [freevars_subst, SUBSET_DEF, IN_DIFF, FDOM_FDIFF]
+  \\ rw [MEM_EL]
+  >>~[‘EL _ (MAP FST _) = EL _ (MAP FST _)’]
+  >- (first_assum $ irule_at Any
+      \\ gvs [EL_MAP]
+      \\ rename1 ‘FST p = FST _’
+      \\ PairCases_on ‘p’
+      \\ fs [])
+  >- (first_assum $ irule_at Any
+      \\ gvs [EL_MAP]
+      \\ rename1 ‘FST p = FST _’
+      \\ PairCases_on ‘p’
+      \\ fs [])
+  \\ first_x_assum $ qspecl_then [‘x’] assume_tac
+  \\ pop_assum kall_tac
+  \\ first_x_assum $ qspecl_then [‘x’] assume_tac
+  \\ gvs [] >>~[‘MEM x (MAP FST l)’]
+  >- (gvs [MEM_EL]
+      \\ first_assum $ irule_at Any
+      \\ fs [EL_MAP]
+      \\ rename1 ‘FST p = FST _’
+      \\ PairCases_on ‘p’ \\ fs [])
+  >- (gvs [MEM_EL]
+      \\ first_assum $ irule_at Any
+      \\ fs [EL_MAP]
+      \\ rename1 ‘FST p = FST _’
+      \\ PairCases_on ‘p’ \\ fs [])
+  \\ first_x_assum $ qspecl_then [‘freevars p'1’] assume_tac
+  \\ gvs [MEM_MAP]
+  \\ pop_assum $ qspecl_then [‘EL k2 l’] assume_tac
+  \\ gvs [EL_MEM]
+QED
+
+Theorem exp_eq_in_ctxt_Prim:
+  ∀c eL eL' ope. LIST_REL (exp_eq_in_ctxt c) eL eL' ⇒ exp_eq_in_ctxt c (Prim ope eL) (Prim ope eL')
+Proof
+  Induct
+  \\ gvs [exp_eq_in_ctxt_def, exp_eq_refl, exp_eq_Prim_cong]
+  \\ rw []
+  \\ irule exp_eq_in_ctxt_trans
+  \\ irule_at Any exp_eq_in_ctxt_trans
+  \\ last_x_assum $ irule_at Any
+  \\ irule_at (Pos last) exp_eq_IMP_exp_eq_in_ctxt
+  \\ irule_at (Pos last) exp_eq_IMP_exp_eq_in_ctxt
+  >~[‘Letrec’]
+  >- (irule_at Any Letrec_Prim
+      \\ irule_at Any $ iffLR exp_eq_sym
+      \\ irule_at Any Letrec_Prim
+      \\ gvs [LIST_REL_EL_EQN, EL_MAP, exp_eq_in_ctxt_def])
+  \\ irule_at Any Let_Prim
+  \\ irule_at Any $ iffLR exp_eq_sym
+  \\ irule_at Any Let_Prim
+  \\ gvs [LIST_REL_EL_EQN, EL_MAP, exp_eq_in_ctxt_def]
+QED
+
+(*
+Theorem freevars_subst1_Let:
+  ∀e n s e1 e2. closed e1 ⇒ freevars (subst1 n (Let s e1 e2) e) = freevars (subst1 n (subst1 s e1 e2) e)
+Proof
+  Induct using freevars_ind
+  \\ rw [subst1_def]
+  >- gvs [freevars_subst1, closed_def]
+  >- (AP_TERM_TAC
+      \\ AP_TERM_TAC
+      \\ irule LIST_EQ
+      \\ rw [EL_MAP]
+      \\ first_x_assum irule
+      \\ fs [EL_MEM])
+  \\ qsuff_tac ‘MAP (FST o (λ(g, z). (g, subst1 n (Let s e1 e2) z))) lcs
+                = MAP (FST o (λ(g, z). (g, subst1 n (subst1 s e1 e2) z))) lcs’
+  >- (rw [MAP_MAP_o]
+      \\ AP_THM_TAC
+      \\ AP_TERM_TAC
+      \\ AP_TERM_TAC
+      \\ AP_TERM_TAC
+      \\ AP_TERM_TAC
+      \\ irule LIST_EQ
+      \\ rw [EL_MAP]
+      \\ rename1 ‘EL k lcs’
+      \\ qabbrev_tac ‘p = EL k lcs’
+      \\ PairCases_on ‘p’
+      \\ fs []
+      \\ first_x_assum irule
+      \\ drule EL_MEM
+      \\ rw []
+      \\ pop_assum $ irule_at Any)
+  \\ irule LIST_EQ
+  \\ rw [EL_MAP]
+  \\ rename1 ‘FST (_ p)’
+  \\ PairCases_on ‘p’
+  \\ fs []
+QED
+
+Theorem subst1_is_Let:
+  ∀e n s e1 e2. closed e1 ⇒ eval (subst1 n (Let s e1 e2) e) = eval (subst1 n (subst1 s e1 e2) e)
+Proof
+  Induct using freevars_ind
+  \\ rw [subst1_def, eval_thm, bind1_def]
+  >- (irule eval_Prim
+      \\ rw [LIST_REL_EL_EQN, EL_MAP]
+      \\ first_x_assum $ irule
+      \\ fs [EL_MEM])
+  >- (TOP_CASE_TAC
+      \\ rename1 ‘dest_Closure _ = SOME x’
+      \\ PairCases_on ‘x’
+      \\ gvs []
+      \\ IF_CASES_TAC
+      \\ gvs [closed_def, freevars_subst1_Let]
+      \\ pop_assum kall_tac
+      \\ first_x_assum $ dxrule_then assume_tac
+      \\ pop_assum $ qspecl_then [‘n’, ‘s’, ‘e2’] assume_tac
+      \\ rw []
+      \\ AP_TERM_TAC \\ AP_TERM_TAC
       \\ cheat)
   \\ cheat
+QED
+
+Theorem Let_App:
+  ∀e1 s e e2. Let s e (App e1 e2) ≈ App (Let s e e1) (Let s e e2)
+Proof
+  rw []
+  \\ irule eval_wh_IMP_exp_eq
+  \\ rw []
+  \\ ‘∀v. v ∈ FRANGE f ⇒ closed v’
+    by (rw []
+        \\ first_x_assum irule
+        \\ fs [FRANGE_FLOOKUP]
+        \\ first_x_assum $ irule_at Any)
+  \\ dxrule_then assume_tac IMP_closed_subst
+  \\ gvs [subst_def, bind1_def, eval_wh_thm]
+  \\ TOP_CASE_TAC \\ fs []
+  \\ rename1 ‘eval_wh (subst1 s (subst f e3) (subst (f \\ s) e1))’
+  \\ Cases_on ‘eval_wh (subst1 s (subst f e3) (subst (f \\ s) e1))’
+  \\ gvs [dest_Closure_def]
+  \\ ‘closed (subst f e3)’
+    by (irule IMP_closed_subst
+            \\ rw []
+        \\ first_x_assum irule
+        \\ fs [FRANGE_FLOOKUP]
+        \\ pop_assum $ irule_at Any)
+  \\ rename1 ‘subst (f \\ s) e2’
+  \\ ‘closed (subst1 s (subst f e3) (subst (f \\ s) e2)) ⇔ freevars (subst (f \\ s) e2) ⊆ {s}’
+    by (drule_then assume_tac closed_freevars_subst1
+        \\ dxrule_then assume_tac closed_subst1_freevars
+        \\ eq_tac \\ strip_tac \\ gvs [])
+  \\ IF_CASES_TAC \\ fs []
+  \\ cheat
+QED*)
+
+Theorem exp_eq_in_ctxt_App:
+  ∀c f1 f2 e1 e2. exp_eq_in_ctxt c f1 f2 ∧ exp_eq_in_ctxt c e1 e2
+                  ⇒ exp_eq_in_ctxt c (App f1 e1) (App f2 e2)
+Proof
+  Induct
+  \\ gvs [exp_eq_in_ctxt_def,exp_eq_App_cong]
+  \\ rw []
+  \\ irule exp_eq_in_ctxt_trans
+  \\ irule_at Any exp_eq_in_ctxt_trans
+  \\ last_x_assum $ irule_at (Pos $ el 2)
+  \\ first_x_assum $ irule_at (Pos $ el 2)
+  \\ rpt $ last_assum $ irule_at Any
+  \\ gvs [exp_eq_IMP_exp_eq_in_ctxt, Let_App, Letrec_App, exp_eq_sym]
+QED
+
+Theorem exp_eq_in_ctxt_Apps:
+  ∀eL eL' e e' c. LIST_REL (exp_eq_in_ctxt c) eL eL' ⇒ exp_eq_in_ctxt c e e'
+                  ⇒ exp_eq_in_ctxt c (Apps e eL) (Apps e' eL')
+Proof
+  Induct
+  >- (Cases
+      \\ fs [Apps_def])
+  \\ gen_tac
+  \\ Cases
+  \\ rw [Apps_def]
+  \\ first_x_assum irule
+  \\ fs [exp_eq_in_ctxt_App]
+QED
+
+Theorem Let_Lam:
+  ∀v w e1 e2. closed e1 ∧ v ≠ w ⇒ Let v e1 (Lam w e2) = Lam w (Let v e1 e2)
+Proof
+  cheat
+QED
+
+Theorem Let_freevars:
+  ∀c v e e'. v ∉ freevars e' ⇒ exp_eq_in_ctxt c (Let v e e') e'
+Proof
+  rw []
+  \\ irule exp_eq_IMP_exp_eq_in_ctxt
+  \\ irule eval_wh_IMP_exp_eq
+  \\ rw [subst_def, eval_wh_thm, bind1_def, GSYM subst_fdomsub]
+  >- (AP_TERM_TAC
+      \\ irule subst1_ignore
+      \\ rename1 ‘subst f e2’
+      \\ qsuff_tac ‘closed (subst f e2)’
+      >- rw [closed_def]
+      \\ irule IMP_closed_subst
+      \\ rw []
+      \\ first_x_assum $ irule_at Any
+      \\ fs [FRANGE_FLOOKUP]
+      \\ pop_assum $ irule_at Any)
+  \\ gvs [IMP_closed_subst, FRANGE_FLOOKUP]
+QED
+
+Theorem exp_eq_in_ctxt_Lam:
+  ∀c v e e'. exp_eq_in_ctxt (IsFree v c) e e' ⇒ exp_eq_in_ctxt c (Lam v e) (Lam v e')
+Proof
+  Induct
+  \\ rw [exp_eq_in_ctxt_def]
+  >- cheat
+  \\ irule exp_eq_in_ctxt_trans
+  \\ irule_at Any exp_eq_in_ctxt_trans
+  >>~[‘Let v _ (Lam w _)’]
+  >- (Cases_on ‘v = w’
+      >- (last_x_assum $ irule_at Any
+          \\ irule_at (Pos last) $ iffLR exp_eq_in_ctxt_sym
+          \\ irule_at (Pos hd) Let_freevars
+          \\ irule_at (Pos last) Let_freevars
+          \\ gvs [exp_eq_in_ctxt_def, freevars_def]
+          \\ rw []
+          \\ irule exp_eq_in_ctxt_trans
+          \\ irule_at Any exp_eq_in_ctxt_trans
+          \\ first_x_assum $ irule_at Any
+          \\ irule_at Any Let_freevars
+          \\ rpt $ first_assum $ irule_at Any
+          \\ irule_at Any $ iffLR exp_eq_in_ctxt_sym
+          \\ gvs [Let_freevars, closed_def])
+      \\ last_x_assum $ irule_at Any
+      \\ fs [exp_eq_in_ctxt_def]
+      \\ cheat)
+  \\ cheat
+QED
+
+Theorem exp_eq_in_ctxt_Lams:
+  ∀vl c e e'. exp_eq_in_ctxt (FOLDL (λc n. IsFree n c) c vl) e e' ⇒
+              exp_eq_in_ctxt c (Lams vl e) (Lams vl e')
+Proof
+  Induct
+  \\ rw [Lams_def]
+  \\ irule exp_eq_in_ctxt_Lam
+  \\ last_x_assum $ irule_at Any
+  \\ fs []
 QED
 
 fun apply_to_first_n 0 tac = ALL_TAC
@@ -1911,14 +2279,14 @@ fun apply_to_first_n 0 tac = ALL_TAC
 
 Theorem find_soundness_lemma:
   ∀e c ds e'. find e c ds e'  ⇒
-                apply_ctxt c e ≈ apply_ctxt c e' ∧
+                exp_eq_in_ctxt c e e' ∧
                 (∀d. d ∈ ds ⇒ e demands d)
 Proof
   Induct_on ‘find’
   \\ rpt conj_tac
   \\ rpt gen_tac
-  >- fs [exp_eq_refl] (* find_Bottom *)
-  >~[‘apply_ctxt c e ≈ apply_ctxt c (Seq (Var v) e2)’] (* find_Seq *)
+  >- fs [exp_eq_in_ctxt_refl] (* find_Bottom *)
+  >~[‘exp_eq_in_ctxt c e (Seq (Var v) e2)’] (* find_Seq *)
   >- (strip_tac
       \\ strip_tac
       \\ fs []
@@ -1926,39 +2294,39 @@ Proof
       \\ rw []
       \\ dxrule_then assume_tac demands_empty_proj
       \\ fs [demands_def, Projs_def]
-      \\ irule exp_eq_apply_ctxt_cong
-      \\ irule exp_eq_trans
+      \\ irule exp_eq_in_ctxt_trans
+      \\ irule_at Any exp_eq_IMP_exp_eq_in_ctxt
       \\ first_assum $ irule_at Any
-      \\ irule exp_eq_Prim_cong
-      \\ fs [exp_eq_refl])
-  >~[‘apply_ctxt c (Seq e e2) ≈ apply_ctxt c (Seq e' e2')’] (* find_Seq2 *)
+      \\ irule exp_eq_in_ctxt_Prim
+      \\ fs [exp_eq_in_ctxt_refl])
+  >~[‘exp_eq_in_ctxt c (Seq e e2) (Seq e' e2')’] (* find_Seq2 *)
   >- (rw []
-      \\ fs [exp_eq_apply_ctxt_cong, exp_eq_Prim_cong, demands_Seq, demands_Seq2])
-  >~[‘apply_ctxt c (If ec et ee) ≈ apply_ctxt c (If ec' et' ee')’]
+      \\ fs [exp_eq_in_ctxt_Prim, demands_Seq, demands_Seq2])
+  >~[‘exp_eq_in_ctxt c (If ec et ee) (If ec' et' ee')’]
   >- (rw []
-      \\ fs [exp_eq_apply_ctxt_cong, demands_If, demands_If2, exp_eq_Prim_cong])
-  >~[‘Var n ≈ Var n’] (* find_Var *)
-  >- fs [exp_eq_apply_ctxt_cong, exp_eq_refl, demands_Var]
-  >~[‘App f e ≈ App f' e'’] (* find_App *)
+      \\ fs [exp_eq_in_ctxt_Prim, demands_If, demands_If2, exp_eq_Prim_cong])
+  >~[‘exp_eq_in_ctxt c (Var n) (Var n)’] (* find_Var *)
+  >- fs [exp_eq_in_ctxt_refl, demands_Var]
+  >~[‘exp_eq_in_ctxt c (App f e) (App f' e')’] (* find_App *)
   >- (rw []
-      \\ fs [exp_eq_apply_ctxt_cong, exp_eq_App_cong, demands_App])
-  >~[‘Apps e el' ≈ Apps e' el''’]
+      \\ fs [exp_eq_in_ctxt_App, demands_App])
+  >~[‘exp_eq_in_ctxt c (Apps e el') (Apps e' el'')’] (* find_Apps *)
   >- (rw []
       \\ fs [Apps_demands]
-      \\ irule exp_eq_Apps_cong
+      \\ irule exp_eq_in_ctxt_Apps
       \\ fs [LIST_REL_EL_EQN]
       \\ rw []
       \\ first_x_assum $ qspecl_then [‘n’] assume_tac
       \\ metis_tac [])
-  >~[‘Proj n i e ≈ Proj n i e'’] (* find_Proj *)
+  >~[‘exp_eq_in_ctxt c (Proj n i e) (Proj n i e')’] (* find_Proj *)
   >- (strip_tac
-      \\ fs [exp_eq_Prim_cong, demands_Proj])
-  >~[‘IsEq n i e ≈ IsEq n i e'’] (* find_IsEq *)
+      \\ fs [exp_eq_in_ctxt_Prim, demands_Proj])
+  >~[‘exp_eq_in_ctxt c (IsEq n i e) (IsEq n i e')’] (* find_IsEq *)
   >- (rw []
-      \\ fs [exp_eq_Prim_cong, demands_IsEq])
-  >~[‘Prim (AtomOp op) el1 ≈ Prim (AtomOp op) el2’]
+      \\ fs [exp_eq_in_ctxt_Prim, demands_IsEq])
+  >~[‘exp_eq_in_ctxt c (Prim (AtomOp op) el1) (Prim (AtomOp op) el2)’] (* find_Atom *)
   >- (rw []
-      >- (irule exp_eq_Prim_cong
+      >- (irule exp_eq_in_ctxt_Prim
           \\ fs [LIST_REL_EL_EQN]
           \\ rw []
           \\ rename1 ‘n < LENGTH _’
@@ -1973,16 +2341,16 @@ Proof
       \\ fs [MEM_EL]
       \\ first_x_assum $ irule_at Any
       \\ fs [])
-  >>~[‘Prim ope el1 ≈ Prim ope el2’] (* find_Prim *)
+  >>~[‘exp_eq_in_ctxt c (Prim ope el1) (Prim ope el2)’] (* find_Prim *)
   >- (rw []
-      \\ irule exp_eq_Prim_cong
+      \\ irule exp_eq_in_ctxt_Prim
       \\ rw [LIST_REL_EL_EQN, EL_MAP]
       \\ rename1 ‘EL n _’
       \\ ‘n < LENGTH el1’ by fs []
       \\ first_x_assum drule
       \\ rw [])
   >- (rw [] (* find_Prim1 *)
-      >- (irule exp_eq_Prim_cong
+      >- (irule exp_eq_in_ctxt_Prim
           \\ rw [LIST_REL_EL_EQN, EL_MAP]
           \\ rename1 ‘EL n _’
           \\ ‘n < LENGTH el1’ by fs []
@@ -1994,12 +2362,14 @@ Proof
       \\ rw []
       \\ Cases_on ‘el1’
       \\ fs [demands_Prim])
-  >~[‘Prim ope el1 ≈ Fail’] (* find_Prim_Fail *)
+  >~[‘exp_eq_in_ctxt c (Prim ope el1) Fail’] (* find_Prim_Fail *)
   >- (rw []
-      \\ fs [not_well_written_is_fail])
-  >>~[‘Let v e e2 ≈ Let v e' e2'’] (* find_Let *)
-  >- (rw []
-      \\ fs [exp_eq_App_cong, exp_eq_Lam_cong]
+      \\ fs [exp_eq_IMP_exp_eq_in_ctxt, not_well_written_is_fail])
+  >>~[‘exp_eq_in_ctxt c (Let v e e2) (Let v e' e2')’] (* find_Let *)
+  >- (rw [exp_eq_in_ctxt_def]
+      >- (irule exp_eq_in_ctxt_trans
+          \\ first_x_assum $ irule_at Any
+          \\ fs [exp_eq_in_ctxt_App, exp_eq_in_ctxt_refl])
       \\ rename1 ‘_ demands d’
       \\ PairCases_on ‘d’
       \\ irule demands_Let2
@@ -2007,8 +2377,10 @@ Proof
       \\ fs []
       \\ last_x_assum irule
       \\ first_x_assum $ irule_at Any)
-  >- (rw []
-      \\ fs [exp_eq_App_cong, exp_eq_Lam_cong]
+  >- (rw [exp_eq_in_ctxt_def]
+      >- (irule exp_eq_in_ctxt_trans
+          \\ first_x_assum $ irule_at Any
+          \\ fs [exp_eq_in_ctxt_App, exp_eq_in_ctxt_refl])
       \\ rename1 ‘_ demands d’
       \\ PairCases_on ‘d’
       \\ first_x_assum dxrule
@@ -2028,14 +2400,10 @@ Proof
       \\ rw []
       \\ drule demands_projs_reduce
       \\ fs [])
-  >- (rw [] (* find_Lam *)
-      \\ fs [exp_eq_Lam_cong])
-  >- (rw []
-      \\ fs [exp_eq_Lams_cong])
-  >- (rw []
-      \\ fs [])
-  >- (rw []
-      \\ fs [exp_eq_Letrec_cong, exp_eq_l_refl])
+  >- rw [exp_eq_in_ctxt_Lam] (* find_Lam *)
+  >- rw [exp_eq_in_ctxt_Lams]
+  >- rw [exp_eq_IMP_exp_eq_in_ctxt]
+  >- rw [exp_eq_in_ctxt_def]
 QED
 
 Theorem find_soundness:
@@ -2043,7 +2411,7 @@ Theorem find_soundness:
 Proof
   rw []
   \\ dxrule find_soundness_lemma
-  \\ fs []
+  \\ fs [exp_eq_in_ctxt_def]
 QED
 
 Datatype:
@@ -2098,7 +2466,7 @@ Definition find_function_def:
   (find_function (Prim op l) c =
   (FEMPTY, Prim op (MAP (λe. SND (find_function e c)) l))) ∧
   (find_function (App (Lam v e2) e) c = let (d, e') = find_function e c in
-                                          let (d2, e2') = find_function e2 (Bind v e c c) in
+                                          let (d2, e2') = find_function e2 (Bind v e c) in
                                            case FLOOKUP d2 v of
                                              | NONE => (d2, App (Lam v e2') e')
                                              | SOME s => (FMERGE merge_dt d (d2 \\ v), Let v e' (Seq (Var v) e2'))) ∧
@@ -2388,7 +2756,7 @@ Proof
        \\ fs [exp_size_def, find_function_def]
        \\ qabbrev_tac ‘ep = find_function e c’
        \\ PairCases_on ‘ep’
-       \\ qabbrev_tac ‘e2p = find_function e2 (Bind s e c c)’
+       \\ qabbrev_tac ‘e2p = find_function e2 (Bind s e c)’
        \\ PairCases_on ‘e2p’
        \\ last_x_assum $ qspecl_then [‘e’] assume_tac
        \\ last_x_assum $ qspecl_then [‘e2’] assume_tac
